updating

case_study/veto_npc.v
@@ -6,7 +6,6 @@ Require Export hetList.
 Require Import ZArith.
 Open Scope Z_scope.
 Require Export Coq.Sets.Ensembles. 
-Require Export Coq.Vectors.VectorDef. 
 
 (*looks nicer in unicode*)
 Definition int := Z. 
@@ -21,105 +20,191 @@ Inductive partition (k:int) (l:list int) : Prop :=
 |partition_ : forall (l1 l2 : list int) , sum l = k * 2 -> Permutation (l1++l2) l ->
                                    sum l1 = k -> sum l2 = k -> partition k l. 
 
-(*list of exactly three elements*)
-Definition vote := t int 3. 
+Inductive voteWF : list int -> int -> Prop := 
+|vetoP : forall k, voteWF [0; k; k] k
+|vetaA : forall k, voteWF [k; 0; k] k
+|vetaB : forall k, voteWF [k; k; 0] k. 
 
-(*shorthand notation for votes*)
-Local Notation " '<<' c1 , c2 , c3 '>>' " := 
-  (cons _ c1 _ (cons _ c2 _ (cons _ c3 _ (nil _)))).
+Definition vote := list int. 
 
-Definition zero_vote := << 0, 0, 0 >>.
-Definition add_votes {n:nat} v1 v2 := @map2 int int int (fun x y => x + y) n v1 v2. 
+Inductive add_votes : vote -> vote -> vote -> Prop :=
+|addNil : add_votes nil nil nil
+|addCons : forall h1 h2 t1 t2 t3,
+             add_votes t1 t2 t3 -> add_votes (h1::t1) (h2::t2) (h1+h2::t3). 
 
-Fixpoint foldVotes vs (base:vote) :=
-  match vs with
-      |v::vs => add_votes v (foldVotes vs base)
-      |List.nil => base
-  end. 
+Inductive fold_votes : list vote -> vote -> Prop :=
+|foldSingle : forall v, fold_votes [v] v
+|foldCons : forall hd tl res res', fold_votes tl res -> add_votes hd res res' ->
+                              fold_votes (hd::tl) res'.
 
 (*The convention here is that the first position corresponds to the 
 **candidate the manipulators want to win << p, a, b >> *)
 Inductive p_wins : vote -> Prop :=
-|p_wins_ : forall hd tl, Forall (fun x => x <= hd) tl -> p_wins (cons _ hd _ tl). 
+|p_wins_ : forall hd tl, Forall (fun x => x <= hd) tl -> p_wins (hd::tl). 
 
-(*base votes correspond to the non-manipulator votes*)
-Inductive manipulate (base_votes : vote) : Prop := 
-|manipulate_ : forall votes, p_wins (foldVotes votes base_votes ) ->
-                        manipulate base_votes. 
+(*base votes correspond to the non-manipulator votes, n is the number of candidates*)
+Inductive manipulate (base_votes : vote) votes : Prop := 
+|manipulate_ : forall res, fold_votes (base_votes::votes) res -> p_wins res ->
+                            Forall (fun v => exists k, voteWF v k) votes ->
+                            manipulate base_votes votes. 
 
 Fixpoint build_veto_a ks :=
   match ks with
-    |k::ks' => List.cons << k*2, 0, k*2 >>(build_veto_a ks')
-    |List.nil => List.nil
+    |k::ks' => [k*2; 0; k*2]::(build_veto_a ks')
+    |nil => [[0;0;0]]
   end. 
 
 Fixpoint build_veto_b ks :=
   match ks with
-    |k::ks' => List.cons << k*2, k*2, 0 >> (build_veto_b ks')
-    |List.nil => List.nil
+    |k::ks' => [k*2; k*2; 0]::(build_veto_b ks')
+    |nil => [[0;0;0]]
   end. 
 
-(*2k-1 votes veto p*)
-Definition reduce k := << 0, k*2-1, k*2-1 >>. 
+Inductive weights : list vote -> list int -> Prop :=
+|nilWeights : weights nil nil
+|consWeights : forall v k vs ks, voteWF v k -> weights vs ks -> 
+                            weights (v::vs) (k::ks). 
+
+Inductive reduce k l : vote -> list vote -> Prop :=
+|reduce_ : forall vs ks, weights vs ks -> Permutation ks l ->
+                    reduce k l [0;k*2-1; k*2-1] vs.
 
 Ltac inv H := inversion H; subst; clear H. 
 
 Theorem sum_veto_a : forall l k, sum l = k -> 
-                            foldVotes (build_veto_a l) zero_vote = << k*2, 0, k*2 >>. 
+                            fold_votes (build_veto_a l) [k*2; 0; k*2]. 
 Proof.
   induction l; intros. 
-  {simpl in *. subst. simpl. reflexivity. }
+  {simpl in *. subst. simpl. constructor. }
   {simpl in H. symmetry in H. apply Zplus_minus_eq in H. apply IHl in H.
-   simpl. rewrite H. simpl. assert(a*2+(k-a)*2 = k*2). omega. rewrite H0.
-   reflexivity. }
+   simpl. econstructor. eauto. assert(k*2=(a*2) + ((k-a)*2)). omega. rewrite H0. 
+   repeat constructor. }
 Qed. 
 
 Theorem sum_veto_b : forall l k, sum l = k -> 
-                            foldVotes(build_veto_b l) zero_vote = << k*2, k*2, 0 >>. 
+                            fold_votes (build_veto_b l) [k*2; k*2; 0].
 Proof.
   induction l; intros. 
-  {inv H. simpl. reflexivity. } 
+  {simpl in *. subst. simpl. constructor. }
   {simpl in H. symmetry in H. apply Zplus_minus_eq in H. apply IHl in H.
-   simpl. rewrite H. simpl. assert(a*2+(k-a)*2 = k*2). omega. rewrite H0. reflexivity. }
+   simpl. econstructor. eauto. assert(k*2=(a*2) + ((k-a)*2)). omega. rewrite H0. 
+   repeat constructor. }
 Qed. 
 
-(*
-Theorem add_veto_a_b : forall l1 l2 l k, Permutation (l1++l2) l -> sum l = k * 2 ->
-                                    sum l1 = k -> sum l2 = k -> 
-                                    add_votes (build_veto_a l1) (build_veto_b l2) =<< k*4, k*2, k*2 >>. 
+Inductive sub_votes : vote -> vote -> vote -> Prop :=
+|subNil : sub_votes [] [] []
+|subCons : forall (h1 h2 : int) (t1 t2 t3 : vote),
+             sub_votes t1 t2 t3 ->
+             sub_votes (h1 :: t1) (h2 :: t2) (h1 - h2 :: t3).
+
+Ltac invertHyp := 
+  match goal with
+      |H:exists x, ?P |- _ => inv H; try invertHyp
+      |H:?A /\ ?B |- _ => inv H; try invertHyp
+  end. 
+
+Ltac copy H :=
+  match type of H with
+      |?x => assert(x) by auto
+  end. 
+
+Theorem addSub : forall a b c d e, 
+                   add_votes a b c -> add_votes c d e ->
+                   exists res, sub_votes e a res. 
 Proof.
-  intros. apply sum_veto_a in H1. rewrite H1. apply sum_veto_b in H2. rewrite H2. 
-  simpl. assert(k*2+k*2 = k*4). omega. rewrite H3. rewrite <- Zplus_0_r_reverse. 
-  reflexivity. 
+  intros. genDeps {{ d; e }}. induction H; intros. 
+  {inv H0. repeat econstructor. }
+  {inv H0. apply IHadd_votes in H5. invertHyp. econstructor. 
+   econstructor. eauto. }
 Qed. 
-*)
 
-Definition shiftout {A} {n:nat} (v:t A (S n)) : t A n :=
-  Eval cbv delta beta in (rectS (fun n _ => t A n) (fun a => @nil A )
-                         (fun h _ _ H => cons _ h _ H) v).
 
-Definition add_votesZero {n:nat} (x:t int (S n)) : t int n :=
-  Eval cbv delta beta in (rectS (fun n _ => t int n) (fun a => @nil int)
-                         (fun h _ _ H => cons _ h _ H) x). 
-
-Theorem _add_votesZero : forall x, add_votes zero_vote x = x. 
+Theorem addSub' : forall a res res1 res2 res3 x, 
+                 add_votes a res res1 -> add_votes res1 res2 res3 ->
+                 sub_votes res3 a x -> add_votes res res2 x. 
 Proof.
-  intros. simpl. apply add_votesZero in x. 
+  intros. genDeps {{ res2;res3;x }}. induction H; intros.
+  {inv H0. inv H1. constructor. }
+  {inv H0. inv H1. assert(h1+h2+h3-h1 = h2+h3). omega. rewrite H0. 
+   constructor. eauto. }
+Qed. 
 
-
-
-Theorem foldVotesApp : forall v1 v2 base, 
-                         foldVotes(v1++v2) base = add_votes (foldVotes v1 zero_vote) (foldVotes v2 base). 
+Theorem addSubEq : forall a b c, sub_votes a b c -> add_votes c b a.
 Proof.
-  induction v1; intros. 
-  {replace (foldVotes [] zero_vote) with zero_vote; auto. 
+  intros. induction H. 
+  {constructor. }
+  {assert((h1-h2)+h2 = h1). omega. rewrite <- H0 at 2. constructor. auto. }
+Qed. 
 
+Theorem add_votes_comm : forall a b c, add_votes a b c -> add_votes b a c. 
+Proof.
+  intros. induction H. 
+  {constructor. }
+  {replace (h1+h2) with (h2+h1). constructor. auto. omega. }
+Qed. 
 
-Theorem veto_npc : forall l (k:int) vs, reduce k = vs ->
-                                 (partition k l <-> manipulate vs). 
+Theorem fold_votes_app : forall a b res1 res2 res3, 
+                           fold_votes a res1 -> 
+                           fold_votes b res2 ->
+                           add_votes res1 res2 res3 -> 
+                           fold_votes (a++b) res3.
+Proof.
+  induction a; intros. 
+  {inv H. }
+  {inv H. 
+   {econstructor. eauto. auto. }
+   {simpl. copy H1. eapply addSub with (a:= a) in H1; eauto. invertHyp. 
+    econstructor. eapply IHa; eauto. eapply addSub'; eauto. 
+    apply add_votes_comm. eapply addSubEq. auto. }
+  }
+Qed. 
+
+Theorem ForallApp : forall (A:Type) P (l1 l2 : list A), 
+                      Forall P l1 -> Forall P l2 -> Forall P (l1++l2).
+Proof.
+  induction l1; intros. 
+  {simpl. auto. }
+  {inv H. simpl. constructor; auto. }
+Qed. 
+
+Theorem build_veto_aWF : forall l, Forall (fun v => exists k, voteWF v k) (build_veto_a l). 
+Proof.
+  induction l; intros. 
+  {simpl. repeat econstructor. }
+  {simpl. repeat econstructor. auto. }
+Qed. 
+
+Theorem build_veto_bWF : forall l, Forall (fun v => exists k, voteWF v k) (build_veto_b l). 
+Proof.
+  induction l; intros. 
+  {simpl. repeat econstructor. }
+  {simpl. repeat econstructor. auto. }
+Qed. 
+
+Theorem veto_npc : forall l (k:int) vs mVs, reduce k l vs mVs ->
+                                     (partition k l <-> manipulate vs mVs). 
 Proof.
   intros. split; intros. 
-  {inversion H0. apply manipulate_ with (votes := build_veto_a l1 ++ build_veto_b l2).
-                         
+  {inversion H0. apply sum_veto_a in H3. apply sum_veto_b in H4.
+   inv H. eapply manipulate_. 
+   eapply manipulate_ with (votes := build_veto_a l1 ++ build_veto_b l2).
+   econstructor. eapply fold_votes_app; eauto. repeat econstructor. 
+   unfold reduce in H. subst. repeat constructor. constructor. 
+   repeat constructor; omega. apply ForallApp. apply build_veto_aWF. 
+   apply build_veto_bWF. }
+  {inv H0. 
+
+
+
+
+
+
+
+
+
+
+
+
+
 
 
